Add inputLines and inputLinesFrom to IO module
I tried to re-use work from the FileIO module, but most of the proof
here was just easier to redo.

The spec for inputLinesFrom is very close to the one in FileIO, so
hopefully the examples can transition to using it without much pain.

basis/fsioSpecScript.sml
@@ -52,6 +52,15 @@ val FST_SPLITP_DROP = Q.store_thm("FST_SPLITP_DROP",
  PURE_REWRITE_TAC[DROP_def,TAKE_def,APPEND] >> simp[] >>
  fs[SPLITP]);
 
+val splitlines_CONS_FST_SPLITP = Q.store_thm("splitlines_CONS_FST_SPLITP",
+  `splitlines ls = ln::lns ⇒ FST (SPLITP ($= #"\n") ls) = ln`,
+  rw[splitlines_def]
+  \\ Cases_on`ls` \\ fs[FIELDS_def]
+  \\ TRY pairarg_tac \\ fs[] \\ rw[] \\ fs[]
+  \\ every_case_tac \\ fs[] \\ rw[] \\ fs[NULL_EQ]
+  \\ qmatch_assum_abbrev_tac`FRONT (x::y) = _`
+  \\ Cases_on`y` \\ fs[]);
+
 val STRCAT_eq = Q.store_thm("STRCAT_eq",
  `∀ x1 x2 y1 y2. LENGTH x1 = LENGTH x2 ∧ x1 ++ y1 = x2 ++ y2 ⇒
     (x1 = x2 ∧ y1 = y2)`,
@@ -956,20 +965,35 @@ val STDIO_numchars = Q.store_thm("STDIO_numchars",
   rw[STDIO_def,GSYM STD_streams_numchars]);
 
 val _ = temp_clear_overloads_on"STRCAT";
+val _ = temp_clear_overloads_on"STRLEN";
+val _ = temp_clear_overloads_on"STRING";
+
+val FDline_def = Define`
+  FDline fs fd = do
+    (content, pos) <- get_file_content fs fd;
+    assert (pos < LENGTH content);
+    let (l,r) = SPLITP ((=)#"\n") (DROP pos content) in
+      SOME(l++"\n") od`;
+
+val bumpLineFD_def = Define`
+  bumpLineFD fs fd =
+    case get_file_content fs fd of
+    | NONE => fs
+    | SOME (content, pos) =>
+      if pos < LENGTH content
+      then let (l,r) = SPLITP ((=)#"\n") (DROP pos content) in
+        (* n.b.: ignores numchars, so only good for STDIO or higher *)
+        bumpFD fd fs (LENGTH l + if NULL r then 0 else 1)
+      else fs`;
 
 val inputLine_spec = Q.store_thm("inputLine_spec",
-  `WORD (n2w fd : word8) fdv ∧ fd ≤ 255 ∧
-   get_file_content fs fd = SOME (content, pos) ∧
-   SPLITP((=)#"\n")(DROP pos content)=(l,r)
+  `WORD (n2w fd : word8) fdv ∧ fd ≤ 255 ∧ IS_SOME (get_file_content fs fd)
    ⇒
    app (p:'ffi ffi_proj) ^(fetch_v "IO.inputLine" (get_ml_prog_state())) [fdv]
      (STDIO fs)
      (POSTv sov.
-       &OPTION_TYPE STRING_TYPE
-         (if pos < LENGTH content
-          then SOME(implode(l++"\n")) else NONE) sov *
-       STDIO (bumpFD fd fs (* ignore numchars because STDIO *)
-                (if pos < LENGTH content then LENGTH l + if NULL r then 0 else 1 else 0)))`,
+       &OPTION_TYPE STRING_TYPE (OPTION_MAP implode (FDline fs fd)) sov *
+       STDIO (bumpLineFD fs fd))`,
   strip_tac
   \\ xcf "IO.inputLine" (basis_st()) >>
   xfun_spec `realloc`
@@ -984,34 +1008,10 @@ val inputLine_spec = Q.store_thm("inputLine_spec",
   xlet_auto >- xsimpl \\
   xlet_auto >- xsimpl \\
   qpat_abbrev_tac`protect = STDIO fs` \\
-  (*
-  xfun_spec `finish`
-    `∀arr n arrv nv.
-      NUM n nv ∧ n ≤ LENGTH arr ⇒
-      app (p:'ffi ffi_proj) finish [arrv;nv]
-        (W8ARRAY arrv arr)
-        (POSTv v.
-          &(OPTION_TYPE STRING_TYPE
-              (if n = 0 then NONE else
-               SOME (implode (MAP (CHR o w2n) (TAKE (n-1) arr) ++ "\n"))) v))`
-  >- (
-    rpt strip_tac
-    \\ first_x_assum match_mp_tac
-    \\ xlet_auto >- xsimpl
-    \\ xif
-    >- ( xcon \\ xsimpl \\ simp[OPTION_TYPE_def] )
-    \\ xlet_auto >- xsimpl
-    \\ xlet_auto >- xsimpl
-    \\ xlet_auto >- xsimpl
-    \\ xcon
-    \\ xsimpl
-    \\ simp[OPTION_TYPE_def,implode_def]
-    \\ fs[STRING_TYPE_def]
-    \\ simp[LIST_EQ_REWRITE,EL_MAP,EL_APPEND_EQN,EL_TAKE,EL_LUPDATE]
-    \\ rw[] \\ fs[] )
-  *)
+  fs[IS_SOME_EXISTS,EXISTS_PROD] \\
+  fs[FDline_def,bumpLineFD_def] \\
+  pairarg_tac \\ fs[] \\
   reverse IF_CASES_TAC \\ fs[] >- (
-    simp[bumpFD_0,STDIO_numchars] \\
     xfun_spec`inputLine_aux`
       `∀arr arrv.
        0 < LENGTH arr ⇒
@@ -1057,6 +1057,7 @@ val inputLine_spec = Q.store_thm("inputLine_spec",
     \\ xapp
     \\ xsimpl ) \\
   qabbrev_tac`arrmax = MAX 128 (2 * LENGTH l + 1)` \\
+  qmatch_assum_rename_tac`get_file_content fs fd = SOME (content,pos)` \\
   xfun_spec `inputLine_aux`
     `∀pp arr i arrv iv fs.
      arr ≠ [] ∧ i ≤ LENGTH arr ∧ LENGTH arr < arrmax ∧
@@ -1101,19 +1102,7 @@ val inputLine_spec = Q.store_thm("inputLine_spec",
       \\ simp[TAKE_APPEND1]
       \\ simp[LEX_DEF]
       \\ Cases_on`LENGTH arr = 0` >- fs[]
-      \\ simp[Abbr`arrmax`]
-      (*
-      \\ `LENGTH arr ≤ LENGTH l` suffices_by fs[]
-      \\ qmatch_assum_rename_tac`x ≤ pos + LENGTH arr`
-      \\ `x = pos + LENGTH arr` by fs[] \\ rveq
-      \\ qpat_x_assum`LENGTH _ < _`mp_tac \\ fs[]
-      \\ imp_res_tac SPLITP_JOIN
-      \\ disch_then kall_tac \\ CCONTR_TAC
-      \\ fs[TAKE_APPEND]
-      \\ imp_res_tac SPLITP_IMP
-      \\ Cases_on`r` \\ fs[]
-      \\ rveq
-      \\ fs[TAKE_LENGTH_TOO_LONG]*))
+      \\ simp[Abbr`arrmax`])
     \\ qmatch_asmsub_rename_tac`MAP _ (TAKE (pp-pos) arr2)`
     \\ qho_match_abbrev_tac`cf_handle _ _ _ _ (POSTv v. post v)`
     \\ reverse (xhandle`POST (λv. &(pp < LENGTH content) * post v)
@@ -1198,7 +1187,6 @@ val inputLine_spec = Q.store_thm("inputLine_spec",
     \\ `pp+1 ≤ LENGTH content` by fs[]
     \\ instantiate
     \\ simp[LEX_DEF]
-    \\ simp[bumpFD_o,STDIO_numchars]
     \\ xsimpl
     \\ fs[ORD_BOUND]
     \\ first_x_assum(qspec_then`_`kall_tac)
@@ -1206,7 +1194,7 @@ val inputLine_spec = Q.store_thm("inputLine_spec",
     >- (
       fs[NULL_EQ]
       \\ imp_res_tac SPLITP_NIL_SND_EVERY
-      \\ rveq \\ fs[]
+      \\ rveq \\ fs[bumpFD_o,STDIO_numchars]
       \\ xsimpl
       \\ `pp + 1 - pos = (pp - pos) + 1` by fs[]
       \\ pop_assum SUBST_ALL_TAC
@@ -1223,7 +1211,7 @@ val inputLine_spec = Q.store_thm("inputLine_spec",
         \\ rw[] )
       \\ simp[DROP_DROP]
       \\ simp[take1_drop,CHAR_EQ_THM] )
-    \\ fs[]
+    \\ fs[bumpFD_o,STDIO_numchars]
     \\ xsimpl
     \\ conj_asm1_tac
     >- (
@@ -1231,9 +1219,8 @@ val inputLine_spec = Q.store_thm("inputLine_spec",
       \\ `pp - pos = LENGTH l` by fs[]
       \\ imp_res_tac SPLITP_JOIN
       \\ fs[NULL_EQ]
-      \\ `EL (pp - pos) (DROP pos content) = HD r`
-      by ( simp[EL_APPEND2] )
-      \\ `pp = STRLEN l + pos` by fs[]
+      \\ `EL (pp - pos) (DROP pos content) = HD r` by ( simp[EL_APPEND2] )
+      \\ `pp = LENGTH l + pos` by fs[]
       \\ `EL pp content = HD r` by (
         qpat_x_assum`_ = HD r` (SUBST1_TAC o SYM)
         \\ simp[EL_DROP] )
@@ -1530,7 +1517,179 @@ val inputLine_spec = Q.store_thm("inputLine_spec",
   qexists_tac`0` >>
   fs[implode_def,bumpFD_def,explode_def] >>
   cheat);
-  *)
 *)
+
+val inputLines_spec = Q.store_thm("input_lines_spec",
+  `WORD ((n2w fd):word8) fdv ∧ fd ≤ 255 ∧
+   get_file_content fs fd = SOME (content,pos)
+   ⇒
+   app (p:'ffi ffi_proj)
+     ^(fetch_v "IO.inputLines"(get_ml_prog_state())) [fdv]
+     (STDIO fs)
+     (POSTv fcv.
+       &LIST_TYPE STRING_TYPE
+         (MAP (\x. strcat (implode x) (implode "\n"))
+            (splitlines (DROP pos content))) fcv *
+       STDIO (bumpFD fd fs (LENGTH content - pos)))`,
+  map_every qid_spec_tac[`fs`] \\
+  Induct_on`splitlines (DROP pos content)` \\ rw[]
+  >- (
+    qpat_x_assum`[] = _`(assume_tac o SYM) \\ fs[DROP_NIL]
+    \\ `LENGTH content - pos = 0` by simp[]
+    \\ pop_assum SUBST1_TAC
+    \\ `DROP pos content = []` by fs[DROP_NIL]
+    \\ fs[bumpFD_0,STDIO_numchars]
+    \\ xcf"IO.inputLines"(get_ml_prog_state())
+    \\ `IS_SOME (get_file_content fs fd)` by fs[IS_SOME_EXISTS]
+    \\ xlet_auto >- xsimpl
+    \\ rfs[FDline_def,OPTION_TYPE_def]
+    \\ xmatch
+    \\ xcon
+    \\ simp[bumpLineFD_def]
+    \\ xsimpl
+    \\ fs[LIST_TYPE_def])
+  \\ qpat_x_assum`_::_ = _`(assume_tac o SYM) \\ fs[]
+  \\ xcf"IO.inputLines"(get_ml_prog_state())
+  \\ `IS_SOME (get_file_content fs fd)` by fs[IS_SOME_EXISTS]
+  \\ xlet_auto >- xsimpl
+  \\ rfs[FDline_def]
+  \\ imp_res_tac splitlines_next
+  \\ rveq
+  \\ `pos < LENGTH content`
+  by ( CCONTR_TAC \\ fs[NOT_LESS,GSYM GREATER_EQ,GSYM DROP_NIL] )
+  \\ fs[DROP_DROP_T]
+  \\ pairarg_tac \\ fs[OPTION_TYPE_def,implode_def,STRING_TYPE_def] \\ rveq
+  \\ xmatch
+  \\ fs[bumpLineFD_def]
+  \\ imp_res_tac splitlines_CONS_FST_SPLITP \\ rfs[] \\ rveq
+  \\ qmatch_goalsub_abbrev_tac`bumpFD fd fs n`
+  \\ first_x_assum(qspecl_then[`pos+n`,`content`]mp_tac)
+  \\ impl_keep_tac
+  >- (
+    simp[Abbr`n`]
+    \\ rw[ADD1]
+    \\ fs[NULL_EQ]
+    \\ imp_res_tac SPLITP_NIL_SND_EVERY
+    \\ rveq
+    \\ simp[DROP_LENGTH_TOO_LONG] )
+  \\ disch_then(qspec_then`bumpFD fd fs n`mp_tac)
+  \\ simp[get_file_content_bumpFD]
+  \\ strip_tac \\ fs[Abbr`n`,NULL_EQ]
+  \\ xlet_auto >- xsimpl
+  \\ xcon
+  \\ xsimpl
+  \\ simp[bumpFD_o,STDIO_numchars,LIST_TYPE_def]
+  \\ fs[strcat_thm,implode_def]
+  \\ qmatch_goalsub_abbrev_tac`pos + n`
+  \\ `n ≤ LENGTH content - pos` suffices_by (simp[] \\ xsimpl)
+  \\ imp_res_tac IS_PREFIX_LENGTH
+  \\ fs[] \\ rw[Abbr`n`] \\ fs[]
+  \\ Cases_on`LENGTH h = LENGTH content - pos` \\ fs[]
+  \\ imp_res_tac SPLITP_JOIN
+  \\ pop_assum(mp_tac o Q.AP_TERM`LENGTH`) \\ simp[]
+  \\ Cases_on`LENGTH r = 0` \\ simp[] \\ fs[] );
+
+val all_lines_def = Define
+  `all_lines fs fname =
+    MAP (\x. strcat (implode x) (implode "\n"))
+          (splitlines (THE (ALOOKUP fs.files fname)))`
+
+val concat_all_lines = Q.store_thm("concat_all_lines",
+  `concat (all_lines fs fname) = implode (THE (ALOOKUP fs.files fname)) ∨
+   concat (all_lines fs fname) = implode (THE (ALOOKUP fs.files fname)) ^ str #"\n"`,
+  rw[all_lines_def] \\
+  qspec_tac(`THE (ALOOKUP fs.files fname)`,`ls`) \\
+  Induct_on`splitlines ls` \\ rw[] \\
+  pop_assum(assume_tac o SYM) \\
+  fs[splitlines_eq_nil,concat_cons]
+  >- EVAL_TAC \\
+  imp_res_tac splitlines_next \\ rw[] \\
+  first_x_assum(qspec_then`DROP (SUC (LENGTH h)) ls`mp_tac) \\
+  rw[] \\ rw[]
+  >- (
+    Cases_on`LENGTH h < LENGTH ls` \\ fs[] >- (
+      disj1_tac \\
+      rw[strcat_thm] \\ AP_TERM_TAC \\
+      fs[IS_PREFIX_APPEND,DROP_APPEND,DROP_LENGTH_TOO_LONG,ADD1] ) \\
+    fs[DROP_LENGTH_TOO_LONG] \\
+    fs[IS_PREFIX_APPEND,strcat_thm] \\ rw[] \\ fs[] \\
+    EVAL_TAC )
+  >- (
+    disj2_tac \\
+    rw[strcat_thm] \\
+    AP_TERM_TAC \\ rw[] \\
+    Cases_on`LENGTH h < LENGTH ls` \\
+    fs[IS_PREFIX_APPEND,DROP_APPEND,ADD1,DROP_LENGTH_TOO_LONG]  \\
+    qpat_x_assum`strlit [] = _`mp_tac \\ EVAL_TAC ));
+
+val _ = overload_on("hasFreeFD",``λfs. CARD (set (MAP FST fs.infds)) ≤ 255``);
+
+val inputLinesFrom_spec = Q.store_thm("inputLinesFrom_spec",
+  `FILENAME f fv /\ hasFreeFD fs
+   ⇒
+   app (p:'ffi ffi_proj) ^(fetch_v"IO.inputLinesFrom"(get_ml_prog_state()))
+     [fv]
+     (STDIO fs)
+     (POSTv sv. &OPTION_TYPE (LIST_TYPE STRING_TYPE)
+            (if inFS_fname fs (File f) then
+               SOME(all_lines fs (File f))
+             else NONE) sv
+             * STDIO fs)`,
+  xcf"IO.inputLinesFrom"(get_ml_prog_state())
+  \\ reverse(xhandle`POST
+       (λv. &OPTION_TYPE (LIST_TYPE STRING_TYPE)
+         (if inFS_fname fs (File f)
+          then SOME(all_lines fs (File f))
+          else NONE) v * STDIO fs)
+       (λe. &(BadFileName_exn e ∧ ¬inFS_fname fs (File f)) * STDIO fs)`)
+  >- (xcases \\ fs[BadFileName_exn_def]
+      \\ reverse conj_tac >- (EVAL_TAC \\ rw[])
+      \\ xcon \\ xsimpl \\ fs[ml_translatorTheory.OPTION_TYPE_def])
+  >- xsimpl
+  \\ `CARD (set (MAP FST fs.infds)) < 256` by fs[]
+  \\ reverse(Cases_on`STD_streams fs`)
+  >- ( fs[STDIO_def] \\ xpull )
+  \\ xlet_auto_spec (SOME (SPEC_ALL openIn_STDIO_spec))
+  >- (
+    xsimpl
+    \\ fs[nextFD_numchars,openFileFS_fupd_numchars,inFS_fname_numchars,GSYM validFD_numchars]
+    \\ CONV_TAC SWAP_EXISTS_CONV
+    \\ qexists_tac`ll` \\ xsimpl )
+  >- (
+    xsimpl
+    \\ rw[inFS_fname_numchars]
+    \\ qexists_tac`ll` \\ xsimpl )
+  \\ drule (GEN_ALL ALOOKUP_inFS_fname_openFileFS_nextFD)
+  \\ imp_res_tac nextFD_leX
+  \\ disch_then(qspec_then`0`mp_tac) \\ rw[]
+  \\ qmatch_assum_abbrev_tac`validFD fd fso`
+  \\ `∃c. get_file_content fso fd = SOME (c,0)`
+  by (
+    fs[get_file_content_def,validFD_def,Abbr`fso`,openFileFS_files]
+    \\ imp_res_tac inFS_fname_ALOOKUP_EXISTS \\ fs[] )
+  \\ xlet_auto >- xsimpl
+  \\ qmatch_goalsub_abbrev_tac`STDIO fsob`
+  \\ qspecl_then[`fd`,`fsob`,`wv`]mp_tac close_STDIO_spec
+  \\ impl_tac >- (
+    fs[STD_streams_def]
+    \\ imp_res_tac ALOOKUP_MEM
+    \\ `¬(fd = 0 ∨ fd = 1 ∨ fd = 2)` suffices_by fs[]
+    \\ metis_tac[nextFD_NOT_MEM] )
+  \\ strip_tac
+  \\ xlet_auto >- xsimpl
+  >- ( xsimpl \\ simp[validFD_bumpFD,Abbr`fsob`] )
+  \\ reverse xcon \\ xsimpl
+  \\ fs[OPTION_TYPE_def]
+  \\ fs[all_lines_def]
+  \\ fs[get_file_content_def]
+  \\ pairarg_tac \\ fs[]
+  \\ fs[Abbr`fso`,openFileFS_files]
+  \\ rveq \\ fs[]
+  \\ qmatch_goalsub_abbrev_tac`STDIO fs'`
+  \\ `∃x. fs' = fs with numchars := x` suffices_by (
+    rw[] \\ rw[STDIO_numchars] \\ xsimpl)
+  \\ unabbrev_all_tac
+  \\ simp[bumpFD_def,A_DELKEY_ALIST_FUPDKEY,o_DEF,
+          IO_fs_component_equality,openFileFS_files]);
 
 val _ = export_theory();
